src/program_logic/crash_inv.v
@@ -29,67 +29,21 @@ Proof. rewrite /Tok. apply _. Qed.
 Definition ci_staged k E1 E2 P : iProp Σ :=
   (|={E1, ∅}=> |={∅, ∅}▷=>^k |={∅, E2}=> P)%I.
 
-Lemma wpc_strong_mono_frame s1 s2 k1 k2 E1 E2 E e Ψ Φc R:
-  s1 ⊑ s2 → k1 ≤ k2 → E1 ⊆ E2 →
-  WPC e @ s1; k1; E1 ; E {{ Ψ }} {{ Φc }} -∗
-  (|={E2,E1}_(k2 - k1)=> R) -∗
-  WPC e @ s2; k2; E2 ; E {{ Ψ }} {{ Φc ∗ R }}.
-Proof.
-  iIntros (?? HE) "H HΦ".
-  iLöb as "IH" forall (e E1 E2 E HE Ψ Φc R).
-  rewrite !wpc_unfold /wpc_pre.
-  iSplit.
-  - destruct (to_val e) as [v|] eqn:?.
-    {
-      iDestruct "H" as "(H&_)".
-      iMod (fupd_intro_mask' _ E1) as "Hclo"; first by auto.
-      iMod "H". iMod "Hclo" as "_". eauto.
-    }
-    iIntros (σ1 κ κs n) "Hσ".
-    iDestruct "H" as "(H&_)".
-    iMod (fupd_intro_mask' _ E1) as "Hclo"; first auto.
-    iMod ("H" with "[$]") as "H".
-    iModIntro.
-    iApply (step_fupdN_le (S k1)); eauto.
-    { lia. }
-    iApply (step_fupdN_wand with "H"). iIntros "H".
-    iMod "H" as "(%&H)".
-      iModIntro.
-      iSplit; [by destruct s1, s2|]. iIntros (e2 σ2 efs Hstep).
-      iMod ("H" with "[//]") as "H". iIntros "!> !>".
-      iMod "H".
-      iMod "Hclo".
-      iModIntro.
-      iApply (step_fupdN_inner_wand with "H"); auto.
-      { lia. }
-      iIntros "(Hσ & H & Hefs)". iFrame.
-      iSplitR "Hefs".
-      ** iApply ("IH" with "[] [H] [HΦ]"); auto.
-      ** iApply (big_sepL_impl with "Hefs"); iIntros "!#" (k ef _).
-         iIntros "H". iApply (wpc_strong_mono' with "H"); eauto.
-  - iDestruct "H" as "(_&H)".
-    replace (S k2) with ((k2 - k1) + (S k1)) by lia.
-    rewrite Nat_iter_add.
-    iMod "HΦ". iModIntro.
-    iApply (step_fupdN_wand with "HΦ"). iIntros "HΦ".
-    iEval (rewrite Nat_iter_S).
-    iMod "HΦ".
-    iMod "H".
-    iApply (step_fupdN_wand with "H"). iIntros "H".
-    iMod "H" as "($&H)". iModIntro. iFrame.
-Qed.
-
-Lemma wpc_ci_inv s k N E1 e Φ Φc P γ :
+(*
+Lemma wpc_ci_inv s k N E1 E2 e Φ Φc P γ :
   ↑N ⊆ E1 →
-  staged_inv N γ (ci_staged (((S (S k)))) (E1 ∖ ↑N) (E1 ∖ ↑N) P) ∗
-  WPC e @ s; (S (S k)); E1; E1 {{ Φ }} {{ Φc }} ⊢
-  WPC e @ s; (2 * (S (S (S k)))); E1; (E1 ∖ ↑N) {{ Φ }} {{ Φc ∗ P }}.
+  ↑N ⊆ E2 →
+  staged_inv N γ (ci_staged (((S (S k)))) (E2 ∖ ↑N) (E2 ∖ ↑N) P) ∗
+  WPC e @ s; (S (S k)); E1; (E2 ∖ ↑N) {{ Φ }} {{ Φc }} ⊢
+  WPC e @ s; (2 * (S (S (S k)))); E1; E2 {{ Φ }} {{ Φc ∗ P }}.
 Proof.
-  iIntros (?) "(#Hinv&H)".
+  iIntros (??) "(#Hinv&H)".
   iApply (wpc_strong_mono s s _ _ E1 _ _ with "H"); try auto.
   { lia. }
-  iModIntro; iSplit; first auto.
+  { set_solver. }
+  iSplit; first auto.
   iIntros "HΦc".
+  replace (E2 ∖ (E2 ∖ ↑N)) with (↑N: coPset).
   iMod (staged_inv_weak_open with "Hinv") as "H"; auto.
   rewrite /ci_staged.
   iMod (fupd_intro_mask' _ ∅) as "Hclo"; first by set_solver+.
@@ -100,7 +54,9 @@ Proof.
   iApply (step_fupdN_inner_wand with "H"); auto.
   iIntros; by iFrame.
 Qed.
+*)
 
+(*
 Lemma wpc_staged_invariant_aux s k E1 E2 E1' E2' e Φ Φc P Q1 R1 Q2 R2 N γ' :
   ↑N ⊆ E1 →
   (E2' ⊆ E1') →
@@ -275,6 +231,7 @@ Proof.
     iMod "H" as "(($&HP)&$)".
     eauto.
 Qed.
+*)
 
 Lemma wpc_staged_invariant s k E1 E2 E1' E2' e Φ Φc Q P N γ :
   ↑N ⊆ E1 →
@@ -282,16 +239,22 @@ Lemma wpc_staged_invariant s k E1 E2 E1' E2' e Φ Φc Q P N γ :
   (E1 ⊆ E1') →
   (E2' ⊆ E2) →
   to_val e = None →
-  staged_inv N γ (ci_staged (2 * (S (S (S k)))) E1' E2' P) ∗
+  staged_inv N γ (ci_staged (2 * (S (S (S k)))) ∅ ∅ P) ∗
   staged_value N γ Q ∗
-  (▷ (Q) -∗ WPC e @ NotStuck; k; (E1 ∖ ↑N); E2
+  (▷ (Q) -∗ WPC e @ NotStuck; k; (E1 ∖ ↑N); ∅
                 {{ λ v, (Φ v ∧ |={E1,E2}=> Φc) ∗ P}} {{ Φc ∗ P }}) ⊢
-  WPC e @ s; (S (S k)); E1; E2 {{ Φ }} {{ Φc }}.
+  WPC e @ s; (S (S k)); E1; ∅ {{ Φ }} {{ Φc }}.
 Proof.
   iIntros (???? Hval) "(#Hinv&Hval&Hwp)".
   rewrite !wpc_unfold /wpc_pre.
   iSplit; last first.
   {
+    (* Actually, should just force you to prove Φc when using the rule, before
+          you get the later ▷ Q, then this rule is trivial *)
+    admit.
+    (*
+    iAssert (|={E1,E1}_(S (S (S k)))=> |={∅,∅}_(S (S (S k)))=> Φc)%I with "[-]" as "H".
+    {
     iMod (staged_inv_open with "[$]") as "(H&Hclo)"; first auto.
     iMod (fupd_intro_mask' _ ∅) as "Hclo'"; first set_solver+.
     iModIntro.
@@ -300,9 +263,15 @@ Proof.
     iMod "Hclo'".
     iApply (step_fupdN_le (S k)); first by set_solver+.
     { lia. }
+    admit.
+    (*
     iApply (step_fupdN_wand with "H").
     iIntros "H". iMod "H" as "(($&?)&$)".
     eauto.
+     *)
+    }
+    admit.
+     *)
   }
   rewrite Hval.
   iIntros (????) "Hstate".
@@ -332,6 +301,7 @@ Proof.
 
     replace (2 * S (S (S k))) with (S (S (S k)) + S (S (S k))) by lia.
     iApply step_fupdN_inner_plus.
+    
     iMod (fupd_intro_mask' _ (E1 ∖ ↑N)) as "Hclo''".
     { set_solver. }
     iMod "H".
